Utils.v
@@ -1,4 +1,4 @@
-Require Import Bool Ascii String AsciiOrder StringOrder List.
+Require Import Bool Arith Ascii String AsciiOrder StringOrder List.
 Import ListNotations.
 Open Scope lazy_bool_scope.
 
@@ -15,15 +15,46 @@ Local Open Scope eqb_scope.
 
 Class Eqb (A : Type) := eqb : A -> A -> bool.
 Infix "=?" := eqb : eqb_scope.
-Arguments eqb {A} _ a a' /.
+Arguments eqb {A} {_} !_ !_.
 
-Instance eqb_inst_nat : Eqb nat := Nat.eqb.
+Class EqbSpec A `{Eqb A} :=
+ eqbspec : forall x y:A, reflect (x=y) (x =? y).
+
+Instance eqb_inst_nat : Eqb nat := { eqb := Nat.eqb }.
+Instance eqbspec_nat : EqbSpec nat := Nat.eqb_spec.
+
 Instance eqb_inst_ascii : Eqb ascii := AsciiOrder.ascii_eqb.
-Instance eqb_inst_string : Eqb string := StringOrder.string_eqb.
+Instance eqbspec_ascii : EqbSpec ascii := AsciiOrder.ascii_eqb_spec.
 
-Arguments eqb_inst_nat /.
-Arguments eqb_inst_ascii /.
-Arguments eqb_inst_string /.
+Instance eqb_inst_string : Eqb string := StringOrder.string_eqb.
+Instance eqbspec_string : EqbSpec string := StringOrder.string_eqb_spec.
+
+Arguments eqb_inst_nat !_ !_.
+Arguments eqb_inst_ascii !_ !_.
+Arguments eqb_inst_string !_ !_.
+
+Lemma eqb_refl {A} `{EqbSpec A} (x:A) : (x =? x) = true.
+Proof.
+ now case eqbspec.
+Qed.
+
+Lemma eqb_eq {A} `{EqbSpec A} (x y:A) : (x =? y) = true <-> x = y.
+Proof.
+ now case eqbspec.
+Qed.
+
+Lemma eqb_neq {A} `{EqbSpec A} (x y:A) : (x =? y) = false <-> x <> y.
+Proof.
+ now case eqbspec.
+Qed.
+
+Lemma eqb_sym {A} `{EqbSpec A} (x y:A) : (x =? y) = (y =? x).
+Proof.
+ case (eqbspec y x); intros.
+ - apply eqb_eq. auto.
+ - apply eqb_neq. auto.
+Qed.
+
 
 Fixpoint list_assoc {A B}`{Eqb A} x (l:list (A*B)) :=
  match l with
@@ -58,16 +89,84 @@ Fixpoint list_max l :=
   | n::l => max n (list_max l)
   end.
 
-
-
 Ltac cons := constructor; congruence.
 
-Lemma forallb2_eqb_spec {A}(eqb : A -> A -> bool) :
- (forall x x', reflect (x=x') (eqb x x')) ->
- forall l l', reflect (l=l') (list_forallb2 eqb l l').
+Instance eqb_inst_list {A}`{Eqb A} : Eqb (list A) := list_forallb2 eqb.
+
+Instance eqbspec_list {A}`{EqbSpec A} : EqbSpec (list A).
 Proof.
- intros EQB.
- induction l; destruct l'; simpl; try cons.
- case EQB; [intros <- | cons].
- case IHl; cons.
+ red.
+ induction x; destruct y; simpl; try cons.
+ cbn.
+ case eqbspec; [ intros <- | cons ].
+ case IHx; cons.
 Defined.
+
+Lemma list_mem_in {A}`{EqbSpec A} (l : list A) x :
+ list_mem x l = true <-> In x l.
+Proof.
+ induction l as [|a l IH]; simpl.
+ - easy.
+ - case eqbspec.
+   + intros <-. intuition discriminate.
+   + rewrite IH. intuition.
+Qed.
+
+Lemma list_assoc_in {A B}`{EqbSpec A} (l : list (A*B)) x :
+ list_assoc x l <> None <-> In x (map fst l).
+Proof.
+ induction l as [|(a,b) l IH]; simpl.
+ - easy.
+ - case eqbspec.
+   + intros <-. intuition discriminate.
+   + rewrite IH. intuition.
+Qed.
+
+Lemma list_assoc_in2 {A B}`{EqbSpec A} (l : list (A*B)) x y :
+ list_assoc x l = Some y -> In (x,y) l.
+Proof.
+ induction l as [|(a,b) l IH]; simpl.
+ - easy.
+ - case eqbspec.
+   + intros <- [= <-]. now left.
+   + intuition.
+Qed.
+
+Lemma list_index_in {A}`{EqbSpec A} (l : list A) x :
+  list_index x l <> None <-> In x l.
+Proof.
+ induction l as [|a l IH]; simpl.
+ - easy.
+ - case eqbspec.
+   + intros <-. intuition discriminate.
+   + destruct list_index; simpl. intuition easy. intuition.
+Qed.
+
+Lemma list_index_nth {A}`{EqbSpec A} (l : list A) n d :
+ NoDup l ->
+ n < List.length l ->
+ list_index (nth n l d) l = Some n.
+Proof.
+ revert n.
+ induction l; simpl.
+ - inversion 2.
+ - intros n. inversion_clear 1.
+   destruct n.
+   + now rewrite eqb_refl.
+   + intros Hn.
+     rewrite IHl; auto with arith; simpl.
+     case eqbspec; auto.
+     intros <-. destruct H2. apply nth_In. auto with arith.
+Qed.
+
+Lemma list_index_lt_length {A}`{EqbSpec A} (l : list A) x n :
+  list_index x l = Some n -> n < List.length l.
+Proof.
+ revert n.
+ induction l; simpl. easy.
+ intros n.
+ case eqbspec.
+ - intros <- [= <-]. auto with arith.
+ - destruct list_index; simpl in *; intros NE [= <-].
+   specialize (IHl n0 eq_refl). auto with arith.
+Qed.
